newErasure/hetList.v
@@ -1,0 +1,16 @@
+  Inductive Het : Type :=
+  |HetConstr : forall A, A -> Het. 
+
+  Inductive hlist : Type :=
+  | HNil : hlist
+  | HCons : forall {A},  A -> hlist -> hlist. 
+
+  Notation "{ x ; .. ; y }" := (HCons x .. (HCons y HNil) ..) : hetlist_scope.
+  Open Scope hetlist_scope. 
+  
+  (*Hack for generalize dependent of multiple parameters*)
+  Ltac genDeps xs :=
+    match xs with
+      |HCons ?x ?xs => generalize dependent x; genDeps xs
+      |HNil => idtac
+    end. 
