newErasure/stepWF.v
@@ -1,0 +1,366 @@
+Require Import NonSpec. 
+Require Import Spec.  
+Require Import Coq.Sets.Ensembles. 
+Require Import erasure. 
+Require Import AST. 
+Require Import SfLib.  
+Require Import hetList. 
+Require Import Coq.Program.Equality. 
+Require Import unspec. 
+Require Import sets. 
+
+Ltac inv H := inversion H; subst; clear H.
+
+Theorem unspecUnionComm : forall T1 T2, unspecPoolAux (tUnion T1 T2) = 
+                                        tUnion (unspecPoolAux T1) (unspecPoolAux T2).
+Proof.
+  intros. apply Extensionality_Ensembles. unfold Same_set. unfold Included. 
+  split; intros. 
+  {inv H. inv H0. inv H2. inv H. 
+   {econstructor. econstructor; eauto. }
+   {apply Union_intror. econstructor; eauto. }
+  }
+  {inv H. 
+   {inv H0. inv H. inv H2. econstructor; eauto. econstructor. econstructor. 
+    eauto. eauto. }
+   {inv H0. inv H. inv H2. econstructor; eauto. econstructor. apply Union_intror. 
+    eauto. eauto. }
+  }
+Qed. 
+
+Theorem multi_trans : forall H T1 T2 H' T1' T2' H'' T1'' T2'', 
+                        multistep H T1 T2 (OK H' T1' T2') -> 
+                        multistep H' T1' T2' (OK H'' T1'' T2'') ->
+                        multistep H T1 T2 (OK H'' T1'' T2''). 
+Proof.
+  intros. genDeps {H''; T1''; T2''}. remember (OK H' T1' T2'). induction H0. 
+  {inv Heqc. intros. auto. }
+  {intros. apply IHmultistep in H2; auto. subst. econstructor; eauto. }
+  {inversion Heqc. }
+Qed. 
+
+
+Theorem unspec_thread : forall t, exists t', unspecThread t (Some t') \/ unspecThread t None. 
+Proof.
+  intros. destruct t. destruct p. destruct p. destruct t0. destruct p. 
+  Admitted. 
+ 
+Ltac eUnspec :=
+  match goal with
+      |H:wellFormed ?H (tUnion ?T (tSingleton ?t)) |- _ => 
+       assert(exists t', unspecThread t (Some t') \/ unspecThread t None)
+         by apply unspec_thread
+  end. 
+
+
+Theorem unspecPoolEmpty : forall t, unspecThread t None -> unspecPoolAux (tSingleton t) = tEmptySet. 
+Proof.
+  intros. apply Extensionality_Ensembles. unfold Same_set. unfold Included. split; intros. 
+  {inversion H0; subst. inversion H1; subst. inversion H3; subst. inversion H4; subst. 
+   clear H3 H4. eapply unspecDeterm in H2; eauto. inversion H2. }
+  {inversion H0. }
+Qed. 
+
+
+Axiom uniqueTP : forall T1 T2 t, tIn (tUnion T1 T2) t -> tIn T1 t -> tIn T2 t -> False. 
+
+Theorem unionEq : forall T1 T2 T2', tUnion T1 T2 = tUnion T1 T2' -> T2 = T2'.  
+Proof.
+  intros. apply Extensionality_Ensembles. unfold Same_set. unfold Included. split; intros. 
+  {apply eqImpliesSameSet in H. unfold Same_set in H. unfold Included in H. inv H. 
+   assert(tIn (tUnion T1 T2) x). apply Union_intror. auto. copy H. apply H1 in H.
+   inversion H; subst. eapply uniqueTP in H0; eauto. inversion H0. auto. }
+  {apply eqImpliesSameSet in H. unfold Same_set in H. unfold Included in H. inv H. 
+   assert(tIn (tUnion T1 T2') x). apply Union_intror. auto. copy H. apply H2 in H3. 
+   inversion H3; subst. eapply uniqueTP in H0; eauto. inversion H0. auto. }
+Qed. 
+
+Hint Constructors Union Couple. 
+
+Theorem coupleUnion : forall X t1 t2, Couple X t1 t2 = Union X (Singleton X t1) (Singleton X t2). 
+Proof.
+  intros. apply Extensionality_Ensembles. unfold Same_set. unfold Included. split; intros. 
+  {inversion H; subst; auto. }
+  {inversion H; subst. inversion H0; subst; auto. inversion H0; subst; auto. }
+Qed. 
+
+
+Theorem moveToUnused : forall t T T' H H', 
+              multistep H tEmptySet (tUnion T (tSingleton t)) (OK H' tEmptySet (tUnion T' (tSingleton t))) <->
+              multistep H (tSingleton t) T (OK H' (tSingleton t) T'). 
+Proof.
+Admitted. 
+
+Ltac replaceWithEmpty :=
+  match goal with
+      |H:multistep ?H (tSingleton ?t) ?T ?x |- _ => 
+       let n := fresh in
+       assert(n:(tSingleton t) = tUnion (tSingleton t) tEmptySet) by (unfold tUnion; rewrite union_empty; auto)
+      | |-multistep ?H (tSingleton ?t) ?T ?x => 
+       let n := fresh in
+       assert(n:(tSingleton t) = tUnion (tSingleton t) tEmptySet) by (unfold tUnion; rewrite union_empty; auto)  
+  end. 
+
+(*Helper theorems for reasoning about the erasure of heaps being rolled back*)
+Theorem unspecHeapRBNew : forall H H' x S A,
+                           unspecHeap H H' ->
+                           Heap.heap_lookup x H = Some(sempty (S::A)) ->
+                           unspecHeap (Heap.remove H x) H'. 
+Proof.
+  induction H; intros. 
+  {simpl in H0. inversion H0. }
+  {simpl in *. destruct a. destruct (beq_nat x i) eqn:eq. 
+   {inversion H1; subst; clear H1. inversion H0; subst. assumption. }
+   {inversion H0; eauto. }
+  }
+Qed. 
+
+Theorem unspecHeapRead :  forall H H' x sc ds ds' S t N,
+                            unspecHeap H H' ->
+                            Heap.heap_lookup x H = Some (sfull sc ds S t N) ->
+                            unspecHeap (Heap.replace x (sfull sc ds' S t N) H) H'. 
+Proof.
+  induction H; intros. 
+  {simpl in *. inversion H0. }
+  {simpl in *. destruct a. destruct (beq_nat x i) eqn:eq. 
+   {inv H1. inversion H0; subst; auto. 
+    {apply beq_nat_true in eq. subst. auto. }
+    {apply beq_nat_true in eq. subst; auto. }
+   }
+   {apply beq_nat_false in eq. inv H0; eauto. }
+  }
+Qed.  
+
+Theorem unspecHeapRBWrite : forall H H' x sc S A tid N,
+                      unspecHeap H H' ->
+                      Heap.heap_lookup x H = Some(sfull sc nil (S::A) tid N) ->
+                      unspecHeap (Heap.replace x (sempty sc) H) H'. 
+Proof.
+  induction H; intros. 
+  {simpl in H0. inversion H0. }
+  {simpl in *. destruct a. destruct (beq_nat x i) eqn:eq. 
+   {inversion H1; subst. clear H1. inversion H0; subst. 
+    econstructor. assumption. apply beq_nat_true in eq. subst. auto. }
+   {inversion H0; eauto. }
+  }
+Qed. 
+
+Theorem unspecHeapWrite : forall H H' x s sc s1 tid M a,
+                            unspecHeap H H' ->
+                            Heap.heap_lookup x H = Some (sempty sc) ->
+                            unspecHeap (Heap.replace x (sfull sc s (a::s1) tid M) H) H'.
+Proof.
+  induction H; intros. 
+  {simpl in *. inversion H0. }
+  {simpl in *. destruct a. destruct (beq_nat x i) eqn:eq. 
+   {apply beq_nat_true in eq; subst. inv H1. inv H0; auto. }
+   {inv H0; auto. }
+  }
+Qed. 
+
+Theorem unspecHeapWriteCommit : forall H H' x s sc tid M,
+                            unspecHeap H H' -> 
+                            Heap.heap_lookup x H = Some (sempty sc) ->
+                            unspecHeap (Heap.replace x (sfull sc s nil tid M) H) 
+                                       (Heap.replace x (sfull sc s nil tid M) H').
+Proof.
+  Admitted. 
+
+
+
+Theorem stepWF : forall H T t H' t', 
+                   wellFormed H (tUnion T t) -> step H T t (OK H' T t') ->
+                   wellFormed H' (tUnion T t'). 
+Proof.
+  intros. inversion H1; subst.   
+  {destruct s1. 
+   {inversion H0; subst. inversion H2; subst. econstructor; eauto. 
+    rewrite unspecUnionComm in *. erewrite unspecSingleton; eauto. 
+    erewrite unspecSingleton in H4; eauto. apply moveToUnused in H4. replaceWithEmpty. 
+    rewrite H in H4. apply multistepUnusedPool in H4. rewrite moveToUnused. replaceWithEmpty. 
+    rewrite H5. rewrite multistepUnusedPool. assumption. }
+   {inversion H0; subst. inversion H2; subst. econstructor; eauto. 
+    rewrite unspecUnionComm in *. eUnspec. invertHyp. inv H5. 
+    {destruct tid. destruct p. erewrite unspecSingleton in *; eauto. Focus 2.
+     erewrite unspecTwoActs. eauto. eapply multi_trans. eauto. econstructor. 
+     eauto.  unfold tUnion. rewrite union_empty. eauto. auto. }
+    {rewrite unspecPoolEmpty in H4; auto. eapply multi_trans. rewrite unspecPoolEmpty. 
+     eassumption. destruct tid. destruct p. erewrite unspecTwoActs. eauto. econstructor. 
+     auto. unfold tUnion. rewrite union_empty. eauto. auto. }
+   }
+  }
+  {destruct s1. 
+   {inversion H0; subst. inversion H2; subst. econstructor; eauto. 
+    rewrite unspecUnionComm in *. erewrite unspecSingleton; eauto. 
+    erewrite unspecSingleton in H4; eauto. apply moveToUnused in H4. replaceWithEmpty. 
+    rewrite H in H4. apply multistepUnusedPool in H4. rewrite moveToUnused. replaceWithEmpty. 
+    rewrite H5. rewrite multistepUnusedPool. assumption. }
+   {inversion H0; subst. inversion H2; subst. econstructor; eauto. 
+    rewrite unspecUnionComm in *. eUnspec. invertHyp. inv H5. 
+    {destruct tid. destruct p. erewrite unspecSingleton in *; eauto. Focus 2.
+     erewrite unspecTwoActs. eauto. eapply multi_trans. eauto. econstructor. 
+     eauto.  unfold tUnion. rewrite union_empty. eauto. auto. }
+    {rewrite unspecPoolEmpty in H4; auto. eapply multi_trans. rewrite unspecPoolEmpty. 
+     eassumption. destruct tid. destruct p. erewrite unspecTwoActs. eauto. econstructor. 
+     auto. unfold tUnion. rewrite union_empty. eauto. auto. }
+   }
+  }
+  {destruct s1. 
+   {inversion H0; subst. inversion H2; subst. econstructor; eauto. 
+    rewrite unspecUnionComm in *. erewrite unspecSingleton; eauto. 
+    erewrite unspecSingleton in H4; eauto. apply moveToUnused in H4. replaceWithEmpty. 
+    rewrite H in H4. apply multistepUnusedPool in H4. rewrite moveToUnused. replaceWithEmpty. 
+    rewrite H5. rewrite multistepUnusedPool. assumption. }
+   {inversion H0; subst. inversion H2; subst. econstructor; eauto. 
+    rewrite unspecUnionComm in *. eUnspec. invertHyp. inv H5. 
+    {destruct tid. destruct p. erewrite unspecSingleton in *; eauto. Focus 2.
+     erewrite unspecTwoActs. eauto. eapply multi_trans. eauto. econstructor. 
+     eauto.  unfold tUnion. rewrite union_empty. eauto. auto. }
+    {rewrite unspecPoolEmpty in H4; auto. eapply multi_trans. rewrite unspecPoolEmpty. 
+     eassumption. destruct tid. destruct p. erewrite unspecTwoActs. eauto. econstructor. 
+     auto. unfold tUnion. rewrite union_empty. eauto. auto. }
+   }
+  }
+  {destruct s1. 
+   {inversion H0; subst. inversion H2; subst. econstructor; eauto. 
+    rewrite unspecUnionComm in *. erewrite unspecSingleton; eauto. 
+    erewrite unspecSingleton in H4; eauto. apply moveToUnused in H4. replaceWithEmpty. 
+    rewrite H in H4. apply multistepUnusedPool in H4. rewrite moveToUnused. replaceWithEmpty. 
+    rewrite H5. rewrite multistepUnusedPool. assumption. }
+   {inversion H0; subst. inversion H2; subst. econstructor; eauto. 
+    rewrite unspecUnionComm in *. eUnspec. invertHyp. inv H5. 
+    {destruct tid. destruct p. erewrite unspecSingleton in *; eauto. Focus 2.
+     erewrite unspecTwoActs. eauto. eapply multi_trans. eauto. econstructor. 
+     eauto.  unfold tUnion. rewrite union_empty. eauto. auto. }
+    {rewrite unspecPoolEmpty in H4; auto. eapply multi_trans. rewrite unspecPoolEmpty. 
+     eassumption. destruct tid. destruct p. erewrite unspecTwoActs. eauto. econstructor. 
+     auto. unfold tUnion. rewrite union_empty. eauto. auto. }
+   }
+  }
+  {destruct s1. 
+   {inversion H0; subst. inversion H2; subst. econstructor; eauto. 
+    rewrite unspecUnionComm in *. erewrite unspecSingleton; eauto. 
+    erewrite unspecSingleton in H4; eauto. apply moveToUnused in H4. replaceWithEmpty. 
+    rewrite H in H4. apply multistepUnusedPool in H4. rewrite moveToUnused. replaceWithEmpty. 
+    rewrite H5. rewrite multistepUnusedPool. assumption. }
+   {inversion H0; subst. inversion H2; subst. econstructor; eauto. 
+    rewrite unspecUnionComm in *. eUnspec. invertHyp. inv H5. 
+    {destruct tid. destruct p. erewrite unspecSingleton in *; eauto. Focus 2.
+     erewrite unspecTwoActs. eauto. eapply multi_trans. eauto. econstructor. 
+     eauto.  unfold tUnion. rewrite union_empty. eauto. auto. }
+    {rewrite unspecPoolEmpty in H4; auto. eapply multi_trans. rewrite unspecPoolEmpty. 
+     eassumption. destruct tid. destruct p. erewrite unspecTwoActs. eauto. econstructor. 
+     auto. unfold tUnion. rewrite union_empty. eauto. auto. }
+   }
+  }
+  {destruct s1. 
+   {inversion H0; subst. inversion H2; subst. econstructor; eauto. 
+    rewrite unspecUnionComm in *. erewrite unspecSingleton; eauto. 
+    erewrite unspecSingleton in H4; eauto. apply moveToUnused in H4. replaceWithEmpty. 
+    rewrite H in H4. apply multistepUnusedPool in H4. rewrite moveToUnused. replaceWithEmpty. 
+    rewrite H5. rewrite multistepUnusedPool. assumption. }
+   {inversion H0; subst. inversion H2; subst. econstructor; eauto. 
+    rewrite unspecUnionComm in *. eUnspec. invertHyp. inv H5. 
+    {destruct tid. destruct p. erewrite unspecSingleton in *; eauto. Focus 2.
+     erewrite unspecTwoActs. eauto. eapply multi_trans. eauto. econstructor. 
+     eauto.  unfold tUnion. rewrite union_empty. eauto. auto. }
+    {rewrite unspecPoolEmpty in H4; auto. eapply multi_trans. rewrite unspecPoolEmpty. 
+     eassumption. destruct tid. destruct p. erewrite unspecTwoActs. eauto. econstructor. 
+     auto. unfold tUnion. rewrite union_empty. eauto. auto. }
+   }
+  }
+  {destruct s1. 
+   {inversion H0; subst. inversion H2; subst. econstructor; eauto. 
+    rewrite unspecUnionComm in *. erewrite unspecSingleton; eauto.  
+    erewrite unspecSingleton in H4; eauto. apply moveToUnused in H4. replaceWithEmpty. 
+    rewrite H in H4. apply multistepUnusedPool in H4. rewrite moveToUnused. replaceWithEmpty. 
+    rewrite H5. rewrite multistepUnusedPool. assumption. }
+   {inversion H0; subst. inversion H2; subst. econstructor; eauto. 
+    rewrite unspecUnionComm in *. eUnspec. invertHyp. inv H5. 
+    {destruct tid. destruct p. erewrite unspecSingleton in *; eauto. Focus 2.
+     erewrite unspecTwoActs. eauto. eapply multi_trans. eauto. econstructor. 
+     eauto.  unfold tUnion. rewrite union_empty. eauto. auto. }
+    {rewrite unspecPoolEmpty in H4; auto. eapply multi_trans. rewrite unspecPoolEmpty. 
+     eassumption. destruct tid. destruct p. erewrite unspecTwoActs. eauto. econstructor. 
+     auto. unfold tUnion. rewrite union_empty. eauto. auto. }
+   }
+  }
+  {inversion H0; subst. inversion H2; subst. econstructor; eauto. unfold tUnion. 
+   rewrite union_empty. rewrite unspecUnionComm in H4. erewrite unspecSingleton in H4; eauto. 
+   apply moveToUnused in H4. replaceWithEmpty. rewrite H in H4. rewrite multistepUnusedPool in H4.
+   auto. }
+  {destruct s1. 
+   {inversion H0; subst. inversion H2; subst. econstructor; eauto. 
+    unfold tCouple. rewrite coupleUnion. repeat rewrite unspecUnionComm in *. 
+    replace (unspecPoolAux(Singleton thread(Tid(1,1)((i,j)::tid),[specAct],[],M))) 
+    with tEmptySet. Focus 2. symmetry. apply unspecPoolEmpty. eapply unspecCreatedSpec; auto. 
+    unfold tUnion. rewrite union_empty. erewrite unspecSingleton. Focus 2. eapply unSpecFork. eauto. 
+    apply decomposeEq in H7. subst. auto. erewrite unspecSingleton in H4; eauto. 
+    eapply multi_trans. apply decomposeEq in H7. subst. eapply H4. 
+    econstructor. auto. unfold tUnion. rewrite union_empty. apply decomposeEq in H7. subst.
+    eauto. rewrite <- coupleUnion. constructor. }
+   {inversion H0; subst. inversion H2; subst. econstructor; eauto. unfold tCouple. 
+    rewrite coupleUnion. repeat rewrite unspecUnionComm in *. 
+    eUnspec. inv H. inversion H5. 
+    {erewrite unspecSingleton. Focus 2. rewrite unspecTwoActs'. eauto. rewrite unspecPoolEmpty. 
+     unfold tUnion. rewrite union_empty. erewrite unspecSingleton in H4; eauto. eapply multi_trans. 
+     eapply H4. econstructor. auto. unfold tUnion. rewrite union_empty. eauto. rewrite <- coupleUnion. 
+     constructor. eauto. }
+    {rewrite unspecPoolEmpty in H4; auto. rewrite unspecPoolEmpty; auto. rewrite unspecPoolEmpty. 
+     unfold tUnion in *. repeat rewrite union_empty in *.  eapply multi_trans. eapply H4. 
+     econstructor. auto. unfold tUnion. rewrite union_empty. eauto. rewrite <- coupleUnion. 
+     constructor. eauto. eauto. rewrite unspecTwoActs'. eauto. }
+   }
+  }
+  {inversion H0; subst. econstructor; eauto. eapply unspecHeapRead; eauto. destruct s1.  
+   {inversion H3; subst. unfold tUnion in *. rewrite unspecUnionComm in *.
+    erewrite unspecSingleton. Focus 2. eapply unspecRead; eauto. apply decomposeEq in H4; subst. 
+    auto. erewrite unspecSingleton in H7; auto. eapply multi_trans. eapply H7. econstructor. auto. 
+    unfold tUnion. rewrite union_empty. eauto. constructor. }
+   {inversion H3; subst. eUnspec. inv H2. inv H8. 
+    {unfold tUnion in *. rewrite unspecUnionComm in *. erewrite unspecSingleton. 
+     Focus 2. simpl. rewrite unspecTwoActs'. eauto. erewrite unspecSingleton in H7; eauto. eapply multi_trans. 
+     eapply H7. econstructor. auto. unfold tUnion. rewrite union_empty. eauto. constructor. }
+    {rewrite unspecUnionComm in *. erewrite unspecPoolEmpty in H7; eauto. 
+     erewrite unspecPoolEmpty. unfold tUnion in*. rewrite union_empty in *. 
+     eapply multi_trans. eapply H7. econstructor. auto. unfold tUnion. rewrite union_empty. 
+     eauto. constructor. simpl. erewrite unspecTwoActs'. eauto. }
+   }
+  }
+  {inversion H0; subst. inversion H3; subst. destruct s1. 
+   {admit. }
+   {eUnspec. inv H2. inv H8. 
+    {econstructor; eauto. eapply unspecHeapWrite; eauto. unfold tUnion in *. 
+     rewrite unspecUnionComm in *. erewrite unspecSingleton. Focus 2. simpl. rewrite unspecTwoActs'. 
+     eauto. erewrite unspecSingleton in H7; eauto. eapply multi_trans. 
+     eapply H7. econstructor. auto. unfold tUnion. rewrite union_empty. eauto. constructor. }
+    {econstructor; eauto. eapply unspecHeapWrite; eauto. rewrite unspecUnionComm in *. 
+     erewrite unspecPoolEmpty in H7; eauto. erewrite unspecPoolEmpty. unfold tUnion in*. 
+     rewrite union_empty in *. eapply multi_trans. eapply H7. econstructor. auto. unfold tUnion. 
+     rewrite union_empty. eauto. constructor. simpl. erewrite unspecTwoActs'. eauto. }
+   }
+  }
+  {(*Overwrite*) admit. }
+  {admit. }
+  {destruct s1. 
+   {inversion H0; subst. inversion H2; subst. econstructor; eauto. 
+    unfold tCouple. rewrite coupleUnion. repeat rewrite unspecUnionComm in *. 
+    erewrite unspecSingleton. Focus 2. eapply unSpecSpecret. eauto. apply decomposeEq in H4. 
+    subst. auto. erewrite unspecPoolEmpty; eauto. unfold tUnion. rewrite union_empty.
+    erewrite unspecSingleton in H5; eauto. eapply multi_trans. apply decomposeEq in H4; subst. 
+    eapply H5. econstructor. auto. unfold tUnion. rewrite union_empty. apply decomposeEq in H4. subst.
+    eauto. rewrite <- coupleUnion. constructor. }
+   {inversion H0; subst. inversion H2; subst. econstructor; eauto. unfold tCouple. 
+    rewrite coupleUnion. repeat rewrite unspecUnionComm in *. 
+    eUnspec. inv H. inv H6. 
+    {erewrite unspecSingleton. Focus 2. simpl. rewrite unspecTwoActs'. eauto. rewrite unspecPoolEmpty. 
+     unfold tUnion. rewrite union_empty. erewrite unspecSingleton in H5; eauto. eapply multi_trans. 
+     eapply H5. econstructor. auto. unfold tUnion. rewrite union_empty. eauto. rewrite <- coupleUnion. 
+     constructor. eauto. }
+    {rewrite unspecPoolEmpty in H5; auto. rewrite unspecPoolEmpty; auto. rewrite unspecPoolEmpty. 
+     unfold tUnion in *. repeat rewrite union_empty in *.  eapply multi_trans. eapply H5. 
+     econstructor. auto. unfold tUnion. rewrite union_empty. eauto. rewrite <- coupleUnion. 
+     constructor. eauto. eauto. simpl. rewrite unspecTwoActs'. eauto. }
+   }
+  }
+  {
